Streamlining of definitions, round 1.
Minor change: the expression and type syntax is now mutually inductive since
Coq's termination checker is rather limited when it comes to nested recursion.

Larger change: I've the typing relation slightly to make it a bit more obvious
that it is indeed functional. Let's look at an example. Below is the typing rule
postfix increment (on numbers).

P; G; S |l- e : qs' ty'
P; G; S |e- e : ty
isReal ty'
isModifiable qs' ty'
---------------------------------- :: PostfixIncrementReal
P; G; S |- incr e : expressionT ty

To type it, we need to check that expression e is of lvalue type, i.e.

(1) P; G; S |l- e : qs' ty'  (note the turnstile annotation),

and we also need to compute its type after lvalue conversion, i.e.

(2) P; G; S |e- e : ty .

Both relations, "|e-" and "|l-", are defined in terms of the top level typing
relation

(3) P; G; S |- e : tc

So a proof of (1) and a proof of (2) both contain a proof of (3) but of course
the type tc should be same in each proof. But that's quite hard to see just from
the definition. Fortunately, whenever we an expression expects a subexpression
to be of lvalue type, we also need to know its expression type. So I have
replaced "|l-" by a relation that combines both "|e-" and "|l-" in the obvious
manner.

ott/coq/AilTypesAux_fun.v
@@ -25,12 +25,11 @@ Definition isPointer_fun t :=
   | _ => false
   end.
 
-Definition isBool_fun it :=
-  match it with
-  | Bool => true
+Definition isBool_fun t :=
+  match t with
+  | Basic (Integer Bool) => true
   | _ => false
   end.
-
 
 Definition isSigned_fun P it : bool :=
   match it with
@@ -154,7 +153,7 @@ Definition eqIntegerRank_fun it1 it2 : bool :=
 
 Definition ltIntegerRankBase_fun P it1 it2 : bool :=
   match it1, it2 with
-  | Bool        , it              => negb (isBool_fun it)
+  | Bool        , it              => negb (bool_of_decision (decide Bool it : Decision (_ = _)))
   | Signed  Long, Signed LongLong => true
   | Signed   Int, Signed     Long => true
   | Signed Short, Signed      Int => true
@@ -393,23 +392,24 @@ Definition isModifiable_fun qs t : bool :=
 
 Definition isReal_fun t : bool := isInteger_fun t.
 
-Definition isLvalueConvertable_fun t : bool := andb (negb (isArray_fun t)) (isComplete_fun t).
+Definition isLvalueConvertible_fun t : bool := andb (negb (isArray_fun t)) (isComplete_fun t).
 
 Fixpoint isCompatible_fun t1 t2 {struct t1} : bool :=
   if bool_of_decision(decide t1 t2 : Decision (t1 = t2)) then
     true
   else
     match t1, t2 with
-    | Function res1 args1, Function res2 args2 =>
-        andb (isCompatible_fun res1 res2) (isCompatible_args_fun args1 args2)
+    | Function t1 p1, Function t2 p2 =>
+        andb (isCompatible_fun t1 t2) (isCompatible_params_fun p1 p2)
     | _, _ => false
     end
-with isCompatible_args_fun args1 args2 : bool :=
-  match args1, args2 with
-  | Argument_nil          , Argument_nil           => true
-  | Argument_nil          , _                      => false
-  | _                     , Argument_nil           => false
-  | Argument_cons _ t1 ls1, Argument_cons _ t2 ls2 => andb (isCompatible_fun t1 t2) (isCompatible_args_fun ls1 ls2)
+with isCompatible_params_fun p1 p2 : bool :=
+  match p1, p2 with
+  | ParamsNil         , ParamsNil          => true
+  | ParamsNil         , _                  => false
+  | _                 , ParamsNil          => false
+  | ParamsCons _ t1 p1, ParamsCons _ t2 p2 => andb (isCompatible_fun        t1 t2)
+                                                   (isCompatible_params_fun p1 p2)
   end.
 
 Fixpoint isComposite_fun t1 t2 t3 : bool :=
@@ -422,16 +422,15 @@ Fixpoint isComposite_fun t1 t2 t3 : bool :=
         andb (andb (bool_of_decision (decide n1 n2 : Decision (n1 = n2)))
                    (bool_of_decision (decide n1 n3 : Decision (n1 = n3))))
              (isComposite_fun t1 t2 t3)
-    | Function t1 l1, Function t2 l2, Function t3 l3 =>
-        andb (isComposite_fun      t1 t2 t3)
-             (isComposite_args_fun l1 l2 l3)
+    | Function t1 p1, Function t2 p2, Function t3 p3 =>
+        andb (isComposite_fun        t1 t2 t3)
+             (isComposite_params_fun p1 p2 p3)
     | _, _, _ => false
     end
-with isComposite_args_fun l1 l2 l3 : bool :=
-  match l1, l2, l3 with
-  | Argument_nil         , Argument_nil         , Argument_nil            => true
-  | Argument_cons _ t1 l1, Argument_cons _ t2 l2, Argument_cons nil t3 l3 =>
-      andb (isComposite_fun      t1 t2 t3)
-           (isComposite_args_fun l1 l2 l3) 
-  | _                    , _                    , _                       => false
+with isComposite_params_fun p1 p2 p3 : bool :=
+  match p1, p2, p3 with
+  | ParamsNil         , ParamsNil         , ParamsNil            => true
+  | ParamsCons _ t1 p1, ParamsCons _ t2 p2, ParamsCons nil t3 p3 => andb (isComposite_fun        t1 t2 t3)
+                                                                         (isComposite_params_fun p1 p2 p3)
+  | _                 , _                 , _                    => false
   end.
