ott/coq/AilSyntaxAux_proof.v
@@ -1,0 +1,37 @@
+Require Import Common.
+Require Import AilTypes.
+Require Import AilSyntax.
+Require Import AilSyntaxAux. 
+Require Import AilSyntaxAux_fun.
+
+Fixpoint fv_fun_correct           id e : boolSpec (fv_fun           id e) (fv           id e)
+with     fv_arguments_fun_correct id l : boolSpec (fv_arguments_fun id l) (fv_arguments id l).
+Proof.
+  + unfold_goal.
+    destruct e;
+    try set (fv_fun_correct id e );
+    try set (fv_fun_correct id e1);
+    try set (fv_fun_correct id e2);
+    try set (fv_fun_correct id e3);
+    try set (fv_arguments_fun_correct id l);
+    my_auto' fail ltac:(progress (bool_simpl; boolSpec_simpl)).
+  + unfold_goal.
+    destruct l;
+    try set (fv_fun_correct id e);
+    try set (fv_arguments_fun_correct id l);
+    my_auto' fail ltac:(progress (bool_simpl; boolSpec_simpl)).
+Defined.
+
+Ltac isNullPointerConstant_fun_tac :=
+  match goal with
+  | [|- boolSpec (isNullPointerConstant_fun ?e) _] =>
+      is_var e; unfold boolSpec; destruct e; simpl; try finish fail; repeat var_destruct
+  end.
+
+Fixpoint isNullPointerConstant_fun_correct e : boolSpec (isNullPointerConstant_fun e) (isNullPointerConstant e).
+Proof.
+  unfold_goal.
+  destruct e; my_auto;
+  set (isNullPointerConstant_fun_correct e);
+  boolSpec_simpl; my_auto.
+Defined.
